agree/agree_compilerScript.sml
@@ -1,0 +1,38 @@
+open HolKernel Parse boolLib bossLib BasicProvers
+     pred_setLib stringLib intLib finite_mapTheory
+     arithmeticTheory listTheory pred_setTheory;
+
+val _ = intLib.prefer_int();
+
+val _ = new_theory "agree_compiler";
+
+
+
+(* ========================================================================== *)
+(* Compilation of a component into a "step" function. The step function       *)
+(* is similar to the semantic componentFn, except that its state              *)
+(* variables are values, not value streams. If                                *)
+(*                                                                            *)
+(*    stepFn = compile comp                                                   *)
+(*                                                                            *)
+(* then it should be the case that the latest values of the streams           *)
+(* computed by iterateFn will be the current values for the state             *)
+(* variables of the stepFn. Roughly:                                          *)
+(*                                                                            *)
+(*  !v. v IN varDecs comp                                                     *)
+(*        ==>                                                                 *)
+(*      !t. (iterateFn E comp t ' v) t =                                      *)
+(*          FUNPOW stepFn t (init_state E) ' v                                *)
+(*                                                                            *)
+(* Some complicating factors:                                                 *)
+(*                                                                            *)
+(*  1. The component needs to be in "pre normal form" so that the state-      *)
+(*     holding variables can be straightforwardly dealt with. The normal form *)
+(*     enforces that the componentFn accesses variable values at most one     *)
+(*     time step back in the stream.                                          *)
+(*                                                                            *)
+(*  2. State variables and output variables are treated the same in E, but    *)
+(*     need to be distinguished in stepFn                                     *)
+(* ========================================================================== *)
+
+val _ = export_theory();
